<?xml version="1.0" encoding="UTF-8"?>
<rdf:RDF
  xmlns:rdf="http://www.w3.org/1999/02/22-rdf-syntax-ns#"
  xmlns:rdfs="http://www.w3.org/2000/01/rdf-schema#"
  xmlns:owl="http://www.w3.org/2002/07/owl#"
  xmlns:vs="http://www.w3.org/2003/06/sw-vocab-status/ns#"
  xmlns:foaf="http://xmlns.com/foaf/0.1/"
  xmlns:dc="http://purl.org/dc/terms/"
  xmlns:time="http://www.w3.org/TR/owl-time#"
  xmlns:vann="http://purl.org/vocab/vann/"
  xmlns:ossr="http://rdfs.genssiz.org/ossr#">


<!-- OSSR Ontology -->
<owl:Ontology rdf:about="http://rdfs.genssiz.org/ossr#" rdf:type="http://www.w3.org/2002/07/owl#Thing">
  <dc:title xml:lang="en">OSSR Ontology Namespace</dc:title>
  <owl:versionInfo>Revision: 0.1</owl:versionInfo>
  <dc:description xml:lang="en">OSSR (Open Semantic Service Relationships) is an ontology developed 
    to describe service networks. It can also be used too simply interlink two or more services.
    The ontology is to be used by Web site about, marketplaces, procurment and outsourcing systems dealing 
	with services. Relationships modeled can be exported (re)construct service networks by external systems. 
  </dc:description>
  <rdfs:seeAlso rdf:resource="http://rdfs.genssiz.org/ossr/spec" rdfs:label="OSSR Ontology Specification"/>
  <foaf:page rdf:resource="http://rdfs.genssiz.org/ossr.html"/>
  <dc:creator rdf:resource="http://rdfs.genssiz.org/ossr#jcardoso"/>
  <dc:modified rdf:datatype="http://www.w3.org/2001/XMLSchema#date">2011-12-12</dc:modified>
  <dc:issued rdf:datatype="http://www.w3.org/2001/XMLSchema#date">2003-06-01</dc:issued>
  <vann:preferredNamespacePrefix>ossr</vann:preferredNamespacePrefix>
  <vann:preferredNamespaceUri>http://rdfs.genssiz.org/ossr#</vann:preferredNamespaceUri>  
</owl:Ontology>

<foaf:Person rdf:about="http://rdfs.genssiz.org/ossr#jcardoso">
  <foaf:name>Jorge Cardoso</foaf:name>
  <foaf:homepage rdf:resource="http://www.jorgecardoso.net"/>
  <foaf:mbox>jcardoso dei uc pt</foaf:mbox>
</foaf:Person>

<foaf:Organization rdf:about="http://rdfs.genssiz.org/ossr#DEI">
  <foaf:member rdf:resource="http://rdfs.genssiz.org/ossr#jcardoso"/>
  <foaf:name>Departement of Engineering Informatics, University of Coimbra, Portugal</foaf:name>
  <foaf:homepage rdf:resource="http://www.dei.uc.pt"/>
</foaf:Organization>


<!-- Classes -->
<owl:Class rdf:about="http://rdfs.genssiz.org/ossr#Relationship" vs:term_status="stable">
  <rdfs:label xml:lang="en">Relationship</rdfs:label>
  <rdfs:comment xml:lang="en">Relationship is a high-level concept that connects two services.</rdfs:comment>
  <rdfs:isDefinedBy rdf:resource="http://rdfs.genssiz.org/ossr"/>
</owl:Class>

<owl:Class rdf:about="http://rdfs.genssiz.org/ossr#Service" vs:term_status="testing">
  <rdfs:label xml:lang="en">Service</rdfs:label>
  <rdfs:comment xml:lang="en">The concept Service represents the two services involved in a relationship and possibly modeled with a language such as Linked-USDL.</rdfs:comment>
  <rdfs:subClassOf rdf:resource="http://www.linked-usdl.org/ns/usdl-core#Service"/>
  <rdfs:isDefinedBy rdf:resource="http://rdfs.genssiz.org/ossr"/>
</owl:Class>

<owl:Class rdf:about="http://rdfs.genssiz.org/ossr#Source">
  <rdfs:label xml:lang="en">Source</rdfs:label>
  <rdfs:comment xml:lang="en">One of the endpoints of the relationship is the service source (Source) and the other one is the service target (Target).</rdfs:comment>
  <rdfs:subClassOf rdf:resource="http://rdfs.genssiz.org/ossr#Service"/>
  <rdfs:isDefinedBy rdf:resource="http://rdfs.genssiz.org/ossr"/>
</owl:Class>

<owl:Class rdf:about="http://rdfs.genssiz.org/ossr#Target">
  <rdfs:label xml:lang="en">Target</rdfs:label>
  <rdfs:comment xml:lang="en">One of the endpoints of the relationship is the service source (Source) and the other one is the service target (Target).</rdfs:comment>
  <rdfs:subClassOf rdf:resource="http://rdfs.genssiz.org/ossr#Service"/>
  <rdfs:isDefinedBy rdf:resource="http://rdfs.genssiz.org/ossr"/>
</owl:Class>

<owl:Class rdf:about="http://rdfs.genssiz.org/ossr#Role">
  <rdfs:label xml:lang="en">Role</rdfs:label>
  <rdfs:comment xml:lang="en">Understanding roles is an important aspect to determine the position of a service in a network. 
  For example, a service can create alliances with complementors to differentiate itself from competition to deliver more value to customers. 
  OSSR specifies four distinct types of roles captured with the concept Role: Customer, Supplier, Competitor, and Complementor.</rdfs:comment>
  <rdfs:isDefinedBy rdf:resource="http://rdfs.genssiz.org/ossr"/>
</owl:Class>

<owl:Class rdf:about="http://rdfs.genssiz.org/ossr#Level">
  <rdfs:label xml:lang="en">Level</rdfs:label>
  <rdfs:comment xml:lang="en">Only the consideration of various levels can led to a sound integration of service layers into networks. 
  Relationships can perform a variety of actions through: Activity links, Actor bonds, and Resource ties.</rdfs:comment>
  <rdfs:isDefinedBy rdf:resource="http://rdfs.genssiz.org/ossr"/>
</owl:Class>

<owl:Class rdf:about="http://rdfs.genssiz.org/ossr#Involvement">
  <rdfs:label xml:lang="en">Involvement</rdfs:label>
  <rdfs:comment xml:lang="en">The concept Involvement represents stakeholders willingness to establish a partnership. 
  Higher levels of involvement usually mean that both parties are more interested to establish a long-term partnership 
  while lower levels of involvement suggest that both parties choose for a more simplified relationship. 
  The concept can take two forms: Low-involvement and High-involvement.
</rdfs:comment>
  <rdfs:isDefinedBy rdf:resource="http://rdfs.genssiz.org/ossr"/>
</owl:Class>

<owl:Class rdf:about="http://rdfs.genssiz.org/ossr#Comparison">
  <rdfs:label xml:lang="en">Comparison</rdfs:label>
  <rdfs:comment xml:lang="en">Comparison consists in the identification of similarities and difierences between services. 
  A service can be described by the functionalities and characteristics it provides (i.e. activities, operations, functions, options, etc.).</rdfs:comment>
  <rdfs:isDefinedBy rdf:resource="http://rdfs.genssiz.org/ossr"/>
</owl:Class>

<owl:Class rdf:about="http://rdfs.genssiz.org/ossr#Association">
  <rdfs:label xml:lang="en">Association</rdfs:label>
  <rdfs:comment xml:lang="en">The association of services enables to combine simpler services into more complex service systems. 
  Associations are a critical building block of many fields of science (e.g. biology, physics, and programming). 
  The concept Association can take the form of: an Aggregation or a Composition.
</rdfs:comment>
  <rdfs:isDefinedBy rdf:resource="http://rdfs.genssiz.org/ossr"/>
</owl:Class>

<owl:Class rdf:about="http://rdfs.genssiz.org/ossr#Causality">
  <rdfs:label xml:lang="en">Causality</rdfs:label>
  <rdfs:comment xml:lang="en">Causality or cause-effect describe how a cause event occurring in a service has an effect in another service. 
  Three concepts model Causality: Cause, Effect, and Link. 
  Causality is expressed using key performance indicators (KPI) of service systems which are connected.</rdfs:comment>
  <rdfs:isDefinedBy rdf:resource="http://rdfs.genssiz.org/ossr"/>
</owl:Class>

<owl:Class rdf:about="http://rdfs.genssiz.org/ossr#Cause">
  <rdfs:label xml:lang="en">Cause</rdfs:label>
  <rdfs:comment xml:lang="en">A key performance indicators (KPI) of service systems which may trigger a cause.</rdfs:comment>
  <rdfs:isDefinedBy rdf:resource="http://rdfs.genssiz.org/ossr"/>
</owl:Class>

<owl:Class rdf:about="http://rdfs.genssiz.org/ossr#Link">
  <rdfs:label xml:lang="en">Link</rdfs:label>
  <rdfs:comment xml:lang="en">The concept Link connects a cause to and sets the sign that a directed link can take: Positive or Negative. A.</rdfs:comment>
  <rdfs:isDefinedBy rdf:resource="http://rdfs.genssiz.org/ossr"/>
</owl:Class>

<owl:Class rdf:about="http://rdfs.genssiz.org/ossr#Effect">
  <rdfs:label xml:lang="en">Effect</rdfs:label>
  <rdfs:comment xml:lang="en">A key performance indicators (KPI) of service systems which is the effect of a cause..</rdfs:comment>
  <rdfs:isDefinedBy rdf:resource="http://rdfs.genssiz.org/ossr"/>
</owl:Class>

		
<!-- Properties -->

<owl:ObjectProperty rdf:about="http://rdfs.genssiz.org/ossr#has_source">
  <rdfs:label xml:lang="en">has_source</rdfs:label>
  <rdfs:comment xml:lang="en">Refers to the source service involved in a service relationship.</rdfs:comment>
  <rdfs:domain rdf:resource="http://rdfs.genssiz.org/ossr#Relationship"/>
  <rdfs:range rdf:resource="http://rdfs.genssiz.org/ossr#Source"/>
  <rdfs:isDefinedBy rdf:resource="http://rdfs.genssiz.org/ossr"/>
</owl:ObjectProperty>

<owl:ObjectProperty rdf:about="http://rdfs.genssiz.org/ossr#has_target">
  <rdfs:label xml:lang="en">has_target</rdfs:label>
  <rdfs:comment xml:lang="en">Refers to the target service involved in a service relationship.</rdfs:comment>
  <rdfs:domain rdf:resource="http://rdfs.genssiz.org/ossr#Relationship"/>
  <rdfs:range rdf:resource="http://rdfs.genssiz.org/ossr#Target"/>
  <rdfs:isDefinedBy rdf:resource="http://rdfs.genssiz.org/ossr"/>
</owl:ObjectProperty>

<owl:ObjectProperty rdf:about="http://rdfs.genssiz.org/ossr#has_service">
  <rdfs:label xml:lang="en">has_target</rdfs:label>
  <rdfs:comment xml:lang="en">Refers to the target service involved in a service relationship.</rdfs:comment>
  <rdfs:domain rdf:resource="http://rdfs.genssiz.org/ossr#Service"/>
  <rdfs:range rdf:resource="http://www.w3.org/TR/rdf-schema/Literal"/>
  <rdfs:isDefinedBy rdf:resource="http://rdfs.genssiz.org/ossr"/>
</owl:ObjectProperty>

<owl:ObjectProperty rdf:about="http://rdfs.genssiz.org/ossr#has_role">
  <rdfs:label xml:lang="en">has_role</rdfs:label>
  <rdfs:comment xml:lang="en">Refers to the role of a service in a relationship: Customer, Supplier, Competitor, Complementor.</rdfs:comment>
  <rdfs:domain rdf:resource="http://rdfs.genssiz.org/ossr#Target"/>
  <rdfs:range rdf:resource="http://www.w3.org/TR/rdf-schema/Literal"/>
  <rdfs:isDefinedBy rdf:resource="http://rdfs.genssiz.org/ossr"/>
</owl:ObjectProperty>

<owl:ObjectProperty rdf:about="http://rdfs.genssiz.org/ossr#has_involvement">
  <rdfs:label xml:lang="en">has_involvement</rdfs:label>
  <rdfs:comment xml:lang="en">Refers to the level of involvement: LowInvolvement or HighInvolvement.</rdfs:comment>
  <rdfs:domain rdf:resource="http://rdfs.genssiz.org/ossr#Relationship"/>
  <rdfs:range rdf:resource="http://www.w3.org/TR/rdf-schema/Literal"/>
  <rdfs:isDefinedBy rdf:resource="http://rdfs.genssiz.org/ossr"/>
</owl:ObjectProperty>

<owl:ObjectProperty rdf:about="http://rdfs.genssiz.org/ossr#has_comparison">
  <rdfs:label xml:lang="en">has_comparison</rdfs:label>
  <rdfs:comment xml:lang="en">Refers to how the services of a relationship are compared from a functional and characteristic point-of-view.
Five comparison operators exist: Equivalent, Generalization, Specialization, Similar, and Different.</rdfs:comment>
  <rdfs:domain rdf:resource="http://rdfs.genssiz.org/ossr#Relationship"/>
  <rdfs:range rdf:resource="http://www.w3.org/TR/rdf-schema/Literal"/>  
  <rdfs:isDefinedBy rdf:resource="http://rdfs.genssiz.org/ossr"/>
</owl:ObjectProperty>

<owl:ObjectProperty rdf:about="http://rdfs.genssiz.org/ossr#has_association">
  <rdfs:label xml:lang="en">has_association</rdfs:label>
  <rdfs:comment xml:lang="en">The association of services enables to combine simpler services into more complex service systems. 
  Associations are a critical building block of many fields of science (e.g. biology, physics, and programming).
Possible values are: AggregationBy, AggregationOf, CompositionBy, and CompositionOf.</rdfs:comment>
  <rdfs:domain rdf:resource="http://rdfs.genssiz.org/ossr#Relationship"/>
  <rdfs:range rdf:resource="http://www.w3.org/TR/rdf-schema/Literal"/>  
  <rdfs:isDefinedBy rdf:resource="http://rdfs.genssiz.org/ossr"/>
</owl:ObjectProperty>

<owl:ObjectProperty rdf:about="http://rdfs.genssiz.org/ossr#has_level">
  <rdfs:label xml:lang="en">has_level</rdfs:label>
  <rdfs:comment xml:lang="en">Refers to the level at which a relationships is established. 
  It can take the values: ActivityLink, ActorBonds, and ResourceTie. </rdfs:comment>
  <rdfs:domain rdf:resource="http://rdfs.genssiz.org/ossr#Relationship"/>
  <rdfs:range rdf:resource="http://www.w3.org/TR/rdf-schema/Literal"/>
  <rdfs:isDefinedBy rdf:resource="http://rdfs.genssiz.org/ossr"/>
</owl:ObjectProperty>

<owl:ObjectProperty rdf:about="http://rdfs.genssiz.org/ossr#has_causality">
  <rdfs:label xml:lang="en">has_causality</rdfs:label>
  <rdfs:comment xml:lang="en">Causality or cause-effect describe how a cause event occurring in a service has an effect in another service. </rdfs:comment>
  <rdfs:domain rdf:resource="http://rdfs.genssiz.org/ossr#Relationship"/>
  <rdfs:range rdf:resource="http://www.w3.org/TR/rdf-schema/Literal"/>
  <rdfs:isDefinedBy rdf:resource="http://rdfs.genssiz.org/ossr"/>
</owl:ObjectProperty>

<owl:ObjectProperty rdf:about="http://rdfs.genssiz.org/ossr#has_cause">
  <rdfs:label xml:lang="en">has_cause</rdfs:label>
  <rdfs:comment xml:lang="en">Refers to the key performance indicators (KPI) of service system which identified the cause.</rdfs:comment>
  <rdfs:domain rdf:resource="http://rdfs.genssiz.org/ossr#Causality"/>
  <rdfs:range rdf:resource="http://rdfs.genssiz.org/ossr#Cause"/>
  <rdfs:isDefinedBy rdf:resource="http://rdfs.genssiz.org/ossr"/>
</owl:ObjectProperty>

<owl:ObjectProperty rdf:about="http://rdfs.genssiz.org/ossr#has_link">
  <rdfs:label xml:lang="en">has_Link</rdfs:label>
  <rdfs:comment xml:lang="en">The concept Link connects a cause to and sets the sign that a directed link can take.</rdfs:comment>
  <rdfs:domain rdf:resource="http://rdfs.genssiz.org/ossr#Causality"/>
  <rdfs:range rdf:resource="http://rdfs.genssiz.org/ossr#Link"/>
  <rdfs:isDefinedBy rdf:resource="http://rdfs.genssiz.org/ossr"/>
</owl:ObjectProperty>

<owl:ObjectProperty rdf:about="http://rdfs.genssiz.org/ossr#has_direction">
  <rdfs:label xml:lang="en">has_Link</rdfs:label>
  <rdfs:comment xml:lang="en">The concept Link connects a cause to and sets the sign that a directed link can take: Positive or Negative. 
  A positive link indicates that a change (increase or decrease) in a service KPI results in the same type of change (increase or decrease) in another service KPI. 
  A negative link indicates that a change (increase or decrease) in a service KPI results in the opposite change (decrease or increase) in another service KPI.</rdfs:comment>
  <rdfs:domain rdf:resource="http://rdfs.genssiz.org/ossr#Link"/>
  <rdfs:range rdf:resource="http://www.w3.org/TR/rdf-schema/Literal"/>
  <rdfs:isDefinedBy rdf:resource="http://rdfs.genssiz.org/ossr"/>
</owl:ObjectProperty>

<owl:ObjectProperty rdf:about="http://rdfs.genssiz.org/ossr#has_effect">
  <rdfs:label xml:lang="en">has_effect</rdfs:label>
  <rdfs:comment xml:lang="en">Refers to the key performance indicators (KPI) of service system which identified the effect.</rdfs:comment>
  <rdfs:domain rdf:resource="http://rdfs.genssiz.org/ossr#Causality"/>
  <rdfs:range rdf:resource="http://rdfs.genssiz.org/ossr#Effect"/>
  <rdfs:isDefinedBy rdf:resource="http://rdfs.genssiz.org/ossr"/>
</owl:ObjectProperty>

<owl:DatatypeProperty rdf:about="http://rdfs.genssiz.org/ossr#has_KPI">
  <rdfs:label xml:lang="en">has_KPI</rdfs:label>
  <rdfs:comment xml:lang="en">Refers to the .</rdfs:comment>
  <rdfs:domain rdf:resource="http://rdfs.genssiz.org/ossr#Cause"/>
  <rdfs:domain rdf:resource="http://rdfs.genssiz.org/ossr#Effect"/>
  <rdfs:range rdf:resource="http://www.w3.org/2001/XMLSchema#anyURI"/>
  <rdfs:isDefinedBy rdf:resource="http://rdfs.genssiz.org/ossr"/>
</owl:DatatypeProperty>
	
<owl:ObjectProperty rdf:about="http://rdfs.genssiz.org/ossr#has_category">
  <rdfs:label xml:lang="en">has_category</rdfs:label>
  <rdfs:comment xml:lang="en">Since KPIs are often domain dependent and their semantics may not always be clear to analysts, individual measures of performance in a cause-effects relation
are classified with a schema composed of five elements: Quality, Time, Cost, Flexibility, Other.</rdfs:comment>
  <rdfs:domain rdf:resource="http://rdfs.genssiz.org/ossr#Cause"/>
  <rdfs:domain rdf:resource="http://rdfs.genssiz.org/ossr#Effect"/>
  <rdfs:range rdf:resource="http://www.w3.org/TR/rdf-schema/Literal"/>
  <rdfs:isDefinedBy rdf:resource="http://rdfs.genssiz.org/ossr"/>
</owl:ObjectProperty>
	

<!-- Management and dynamic support -->

<owl:DatatypeProperty rdf:about="http://rdfs.genssiz.org/ossr#has_validity">
  <rdfs:label xml:lang="en">has_validity</rdfs:label>
  <rdfs:comment xml:lang="en">The interval of time during which the relationship model is valid.
  </rdfs:comment>
  <rdfs:domain rdf:resource="http://rdfs.genssiz.org/ossr#Relationship"/>
  <rdfs:range rdf:resource="http://www.w3.org/TR/owl-time#Interval"/>
  <rdfs:isDefinedBy rdf:resource="http://rdfs.genssiz.org/ossr"/>
</owl:DatatypeProperty>
 
</rdf:RDF>
